ironfleet/src/Dafny/Distributed/Services/RSL/AppStateMachine.s.dfy
@@ -1,16 +1,44 @@
 include "../../Common/Native/Io.s.dfy"
 
-abstract module AppStateMachine_s {
+module AppStateMachine_s {
 import opened Native__NativeTypes_s
 import opened Native__Io_s
 
-type AppState
-type AppMessage 
+type Bytes = seq<byte>
+type AppState = Bytes
+type AppRequest = Bytes
+type AppReply = Bytes
 
-function AppInitialize() : AppState
-predicate AppValidRequest(request:AppMessage)
-function AppHandleRequest(m:AppState, request:AppMessage) : (AppState, AppMessage)
+function {:axiom} AppInitialize() : AppState
+function {:axiom} AppHandleRequest(m:AppState, request:AppRequest) : (AppState, AppReply)
+function method MaxAppRequestSize() : int  { 0x800_0000 }            // 128 MB
+function method MaxAppReplySize() : int    { 0x800_0000 }            // 128 MB
+function method MaxAppStateSize() : int    { 0x1000_0000_0000_0000 } // 2^60 B
 
-function MarshallAppMessage(m:AppMessage) : seq<byte>
+class AppStateMachine
+{
+  constructor{:axiom} ()
+    requires false
+
+  function {:axiom} Abstractify() : AppState
+
+  static method {:axiom} Initialize() returns (m:AppStateMachine)
+    ensures fresh(m)
+    ensures m.Abstractify() == AppInitialize()
+
+  static method {:axiom} Deserialize(state:AppState) returns (m:AppStateMachine)
+    ensures fresh(m)
+    ensures m.Abstractify() == state
+
+  method {:axiom} Serialize() returns (state:AppState)
+    ensures state == Abstractify()
+    ensures |state| <= MaxAppStateSize()
+
+  method {:axiom} HandleRequest(request:AppRequest) returns (reply:AppReply)
+    requires |request| <= MaxAppRequestSize()
+    ensures  (Abstractify(), reply) == AppHandleRequest(old(Abstractify()), request)
+    ensures  |reply| <= MaxAppReplySize()
+}
+
 }
 
