ironfleet/src/Dafny/Distributed/Impl/RSL/CMessageRefinements.i.dfy
@@ -24,15 +24,15 @@ predicate CMessageIsAbstractable(msg:CMessage)
 {
   match msg
     case CMessage_Invalid => true
-    case CMessage_Request(seqno, value) => CAppMessageIsAbstractable(value)
+    case CMessage_Request(seqno, value) => CAppRequestIsAbstractable(value)
     case CMessage_1a(ballot) => CBallotIsAbstractable(ballot)
     case CMessage_1b(ballot, log_truncation_point, votes) => CBallotIsAbstractable(ballot) && COperationNumberIsAbstractable(log_truncation_point) && CVotesIsAbstractable(votes)
     case CMessage_2a(ballot, opn, value) => CBallotIsAbstractable(ballot) && COperationNumberIsAbstractable(opn) && CRequestBatchIsAbstractable(value)
     case CMessage_2b(ballot, opn, value) => CBallotIsAbstractable(ballot) && COperationNumberIsAbstractable(opn) && CRequestBatchIsAbstractable(value)
     case CMessage_Heartbeat(bal_heartbeat, suspicious, opn_ckpt) => CBallotIsAbstractable(bal_heartbeat) && COperationNumberIsAbstractable(opn_ckpt)
-    case CMessage_Reply(seqno, reply) => CAppMessageIsAbstractable(reply)
+    case CMessage_Reply(seqno, reply) => CAppReplyIsAbstractable(reply)
     case CMessage_AppStateRequest(bal_state_req, opn_state_req) => CBallotIsAbstractable(bal_state_req) && COperationNumberIsAbstractable(opn_state_req)
-    case CMessage_AppStateSupply(bal_state_supply, opn_state_supply, app_state, reply_cache) => CBallotIsAbstractable(bal_state_supply) && COperationNumberIsAbstractable(opn_state_supply) && CTransferableAppStateIsAbstractable(app_state) && CReplyCacheIsAbstractable(reply_cache)
+    case CMessage_AppStateSupply(bal_state_supply, opn_state_supply, app_state, reply_cache) => CBallotIsAbstractable(bal_state_supply) && COperationNumberIsAbstractable(opn_state_supply) && CAppStateIsAbstractable(app_state) && CReplyCacheIsAbstractable(reply_cache)
     case CMessage_StartingPhase2(bal_2, logTruncationPoint_2) => CBallotIsAbstractable(bal_2) && COperationNumberIsAbstractable(logTruncationPoint_2)
 
 }
@@ -42,15 +42,15 @@ function AbstractifyCMessageToRslMessage(msg:CMessage) : RslMessage
 {
   match msg
     case CMessage_Invalid => RslMessage_Invalid()
-    case CMessage_Request(seqno, value) => RslMessage_Request(seqno as int, AbstractifyCAppMessageToAppMessage(value))
+    case CMessage_Request(seqno, value) => RslMessage_Request(seqno as int, AbstractifyCAppRequestToAppRequest(value))
     case CMessage_1a(ballot) => RslMessage_1a(AbstractifyCBallotToBallot(ballot))
     case CMessage_1b(ballot, log_truncation_point, votes) => RslMessage_1b(AbstractifyCBallotToBallot(ballot), AbstractifyCOperationNumberToOperationNumber(log_truncation_point), AbstractifyCVotesToVotes(votes))
     case CMessage_2a(ballot, opn, value) => RslMessage_2a(AbstractifyCBallotToBallot(ballot), AbstractifyCOperationNumberToOperationNumber(opn), AbstractifyCRequestBatchToRequestBatch(value))
     case CMessage_2b(ballot, opn, value) => RslMessage_2b(AbstractifyCBallotToBallot(ballot), AbstractifyCOperationNumberToOperationNumber(opn), AbstractifyCRequestBatchToRequestBatch(value))
     case CMessage_Heartbeat(bal_heartbeat, suspicious, opn_ckpt) => RslMessage_Heartbeat(AbstractifyCBallotToBallot(bal_heartbeat), suspicious, AbstractifyCOperationNumberToOperationNumber(opn_ckpt))
-    case CMessage_Reply(seqno, reply) => RslMessage_Reply(seqno as int, AbstractifyCAppMessageToAppMessage(reply))
+    case CMessage_Reply(seqno, reply) => RslMessage_Reply(seqno as int, AbstractifyCAppReplyToAppReply(reply))
     case CMessage_AppStateRequest(bal_state_req, opn_state_req) => RslMessage_AppStateRequest(AbstractifyCBallotToBallot(bal_state_req), AbstractifyCOperationNumberToOperationNumber(opn_state_req))
-    case CMessage_AppStateSupply(bal_state_supply, opn_state_supply, app_state, reply_cache) => RslMessage_AppStateSupply(AbstractifyCBallotToBallot(bal_state_supply), AbstractifyCOperationNumberToOperationNumber(opn_state_supply), AbstractifyCTransferableAppStateToAppState(app_state), AbstractifyCReplyCacheToReplyCache(reply_cache))
+    case CMessage_AppStateSupply(bal_state_supply, opn_state_supply, app_state, reply_cache) => RslMessage_AppStateSupply(AbstractifyCBallotToBallot(bal_state_supply), AbstractifyCOperationNumberToOperationNumber(opn_state_supply), AbstractifyCAppStateToAppState(app_state), AbstractifyCReplyCacheToReplyCache(reply_cache))
     case CMessage_StartingPhase2(bal_2, logTruncationPoint_2) => RslMessage_StartingPhase2(AbstractifyCBallotToBallot(bal_2), AbstractifyCOperationNumberToOperationNumber(logTruncationPoint_2))
 }
 
