ironfleet/src/Dafny/Distributed/Impl/RSL/PacketParsing.i.dfy
@@ -6,7 +6,6 @@ include "../Common/GenericMarshalling.i.dfy"
 include "CTypes.i.dfy"
 include "CMessage.i.dfy"
 include "CMessageRefinements.i.dfy"
-include "AppInterface.i.dfy"
 
 module LiveRSL__PacketParsing_i {
 import opened Native__Io_s
@@ -24,6 +23,7 @@ import opened Common__GenericMarshalling_i
 import opened Common__NodeIdentity_i
 import opened Common__UdpClient_i
 import opened Common__Util_i
+import opened AppStateMachine_s
 import opened Environment_s
 import opened Math__mul_i
 import opened Math__mul_nonlinear_i
@@ -32,9 +32,9 @@ import opened Math__mul_nonlinear_i
 //    Grammars for the Paxos types
 ////////////////////////////////////////////////////////////////////
 function method EndPoint_grammar() : G { GUint64 }
-function method CRequest_grammar() : G { GTuple([EndPoint_grammar(), GUint64, CAppMessage_grammar()]) }
+function method CRequest_grammar() : G { GTuple([EndPoint_grammar(), GUint64, GByteArray]) }
 function method CRequestBatch_grammar() : G { GArray(CRequest_grammar()) }
-function method CReply_grammar() : G { GTuple([EndPoint_grammar(), GUint64, CAppMessage_grammar()]) }
+function method CReply_grammar() : G { GTuple([EndPoint_grammar(), GUint64, GByteArray]) }
 function method CBallot_grammar() : G { GTuple([GUint64, GUint64]) }
 function method COperationNumber_grammar() : G { GUint64 }
 function method CVote_grammar() : G { GTuple([CBallot_grammar(), CRequestBatch_grammar()])} 
@@ -45,15 +45,15 @@ function method CReplyCache_grammar() : G { GArray(GTuple([EndPoint_grammar(), C
 ////////////////////////////////////////////////////////////////////
 //    Grammars for the Paxos messages 
 ////////////////////////////////////////////////////////////////////
-function method CMessage_Request_grammar() : G { GTuple([GUint64, CAppMessage_grammar()]) }
+function method CMessage_Request_grammar() : G { GTuple([GUint64, GByteArray]) }
 function method CMessage_1a_grammar() : G { CBallot_grammar() }
 function method CMessage_1b_grammar() : G { GTuple([CBallot_grammar(), COperationNumber_grammar(), CVotes_grammar()]) }
 function method CMessage_2a_grammar() : G { GTuple([CBallot_grammar(), COperationNumber_grammar(), CRequestBatch_grammar()]) }
 function method CMessage_2b_grammar() : G { GTuple([CBallot_grammar(), COperationNumber_grammar(), CRequestBatch_grammar()]) }
 function method CMessage_Heartbeat_grammar() : G { GTuple([CBallot_grammar(), GUint64, COperationNumber_grammar()]) }
-function method CMessage_Reply_grammar() : G { GTuple( [GUint64, CAppMessage_grammar()] ) }
+function method CMessage_Reply_grammar() : G { GTuple( [GUint64, GByteArray] ) }
 function method CMessage_AppStateRequest_grammar() : G { GTuple([CBallot_grammar(), COperationNumber_grammar()]) }
-function method CMessage_AppStateSupply_grammar() : G { GTuple([CBallot_grammar(), COperationNumber_grammar(), CTransferableAppState_grammar(), CReplyCache_grammar()]) }
+function method CMessage_AppStateSupply_grammar() : G { GTuple([CBallot_grammar(), COperationNumber_grammar(), GByteArray, CReplyCache_grammar()]) }
 function method CMessage_StartingPhase2_grammar() : G { GTuple([CBallot_grammar(), COperationNumber_grammar()]) }
 
 function method CMessage_grammar() : G { GTaggedUnion([
@@ -137,7 +137,7 @@ function method parse_Request(val:V) : CRequest
   assert ValInGrammar(val.t[1], CRequest_grammar().t[1]);      // OBSERVE 
   assert ValInGrammar(val.t[2], CRequest_grammar().t[2]);      // OBSERVE 
   var ep := parse_EndPoint(val.t[0]);
-  CRequest(ep, val.t[1].u, parse_AppMessage(val.t[2]))
+  CRequest(ep, val.t[1].u, val.t[2].b)
 }
 
 function parse_RequestBatch(val:V) : CRequestBatch
@@ -210,7 +210,7 @@ function method parse_Reply(val:V) : CReply
   assert ValInGrammar(val.t[1], CReply_grammar().t[1]);      // OBSERVE 
   assert ValInGrammar(val.t[2], CReply_grammar().t[2]);      // OBSERVE 
   var ep := parse_EndPoint(val.t[0]);
-  CReply(ep, val.t[1].u, parse_AppMessage(val.t[2]))
+  CReply(ep, val.t[1].u, val.t[2].b)
 }
 
 function method parse_Ballot(val:V) : CBallot
@@ -357,7 +357,7 @@ function method parse_Message_Request(val:V) : CMessage
 {
   assert ValInGrammar(val.t[0], CMessage_Request_grammar().t[0]);      // OBSERVE
   assert ValInGrammar(val.t[1], CMessage_Request_grammar().t[1]);      // OBSERVE
-  CMessage_Request(val.t[0].u, parse_AppMessage(val.t[1]))
+  CMessage_Request(val.t[0].u, val.t[1].b)
 }
 
 function method parse_Message_1a(val:V) : CMessage
@@ -440,7 +440,7 @@ function method parse_Message_Reply(val:V) : CMessage
 {
   assert ValInGrammar(val.t[0], CMessage_Reply_grammar().t[0]);      // OBSERVE
   assert ValInGrammar(val.t[1], CMessage_Reply_grammar().t[1]);      // OBSERVE
-  CMessage_Reply(val.t[0].u, parse_AppMessage(val.t[1]))
+  CMessage_Reply(val.t[0].u, val.t[1].b)
 }
 
 function method parse_Message_AppStateRequest(val:V) : CMessage
@@ -456,7 +456,8 @@ function method parse_Message_AppStateSupply(val:V) : CMessage
   ensures  CMessageIsAbstractable(parse_Message_AppStateSupply(val))
   ensures  ValidVal(val) ==> CMessageIs64Bit(parse_Message_AppStateSupply(val))
 {
-  CMessage_AppStateSupply(parse_Ballot(val.t[0]), parse_OperationNumber(val.t[1]), parse_TransferableAppState(val.t[2]), parse_ReplyCache(val.t[3]))
+  assert ValInGrammar(val.t[2], GByteArray);
+  CMessage_AppStateSupply(parse_Ballot(val.t[0]), parse_OperationNumber(val.t[1]), val.t[2].b, parse_ReplyCache(val.t[3]))
 }
 
 function method parse_Message_StartingPhase2(val:V) : CMessage
@@ -582,15 +583,15 @@ function Marshallable_2b(msg:CMessage) : bool
 function Marshallable(msg:CMessage) : bool
 {
   && (!msg.CMessage_Invalid?)
-  && (msg.CMessage_Request? ==> ValidCAppMessage(msg.val))
+  && (msg.CMessage_Request? ==> CAppRequestMarshallable(msg.val))
   && (msg.CMessage_1a? ==> true)
   && (msg.CMessage_1b? ==> ValidVotes(msg.votes))
   && (msg.CMessage_2a? ==> Marshallable_2a(msg))
   && (msg.CMessage_2b? ==> Marshallable_2b(msg))
   && (msg.CMessage_Heartbeat? ==> true)
-  && (msg.CMessage_Reply? ==> ValidCAppMessage(msg.reply))
+  && (msg.CMessage_Reply? ==> CAppReplyMarshallable(msg.reply))
   && (msg.CMessage_AppStateRequest? ==> true)
-  && (msg.CMessage_AppStateSupply? ==> TransferableAppStateMarshallable(msg.app_state) && ValidReplyCache(msg.reply_cache))
+  && (msg.CMessage_AppStateSupply? ==> CAppStateMarshallable(msg.app_state) && ValidReplyCache(msg.reply_cache))
   && (msg.CMessage_StartingPhase2? ==> true)
 }
 
@@ -621,7 +622,7 @@ method DetermineIfValidVote(vote:CVote) returns (b:bool)
     invariant forall i :: 0 <= i < pos ==> ValidRequest(vote.max_val[i])
   {
     var c := vote.max_val[pos];
-    if c.CRequest? && !ValidCAppMessage(c.request) {
+    if c.CRequest? && !CAppRequestMarshallable(c.request) {
       assert !ValidRequest(c);
       assert !ValidRequestBatch(vote.max_val);
       b := false;
@@ -683,7 +684,7 @@ method DetermineIfValidReplyCache(m:CReplyCache) returns (b:bool)
     var e :| e in keys;
     assert EndPointIsValidIPV4(e);
     assert CReplyIsAbstractable(m[e]);
-    if m[e].CReply? && !ValidCAppMessage(m[e].reply) {
+    if m[e].CReply? && !CAppReplyMarshallable(m[e].reply) {
       b := false;
       assert !ValidReply(m[e]);
       return;
@@ -726,7 +727,7 @@ method DetermineIfMessageMarshallable(msg:CMessage) returns (b:bool)
     b := false;
   }
   else if msg.CMessage_Request? {
-    b := ValidCAppMessage(msg.val);
+    b := CAppRequestMarshallable(msg.val);
   }
   else if msg.CMessage_1a? {
     b := true;
@@ -744,13 +745,13 @@ method DetermineIfMessageMarshallable(msg:CMessage) returns (b:bool)
     b := true;
   }
   else if msg.CMessage_Reply? {
-    b := ValidCAppMessage(msg.reply);
+    b := CAppReplyMarshallable(msg.reply);
   }
   else if msg.CMessage_AppStateRequest? {
     b := true;
   }
   else if msg.CMessage_AppStateSupply? {
-    var b1 := TransferableAppStateMarshallable(msg.app_state);
+    var b1 := CAppStateMarshallable(msg.app_state);
     var b2 := DetermineIfValidReplyCache(msg.reply_cache);
     b := b1 && b2;
   }
@@ -782,7 +783,7 @@ method MarshallRequest(c:CRequest) returns (val:V)
   ensures  ValidVal(val)
   ensures  parse_Request(val) == c
 {
-  var marshalled_app_message := MarshallCAppMessage(c.request);
+  var marshalled_app_message := MarshallCAppRequest(c.request);
   var marshalled_ep := MarshallEndPoint(c.client);
   val := VTuple([marshalled_ep, VUint64(c.seqno), marshalled_app_message]);
 
@@ -825,7 +826,7 @@ method MarshallReply(c:CReply) returns (val:V)
   ensures  ValidVal(val)
   ensures  parse_Reply(val) == c
 {
-  var marshalled_app_message := MarshallCAppMessage(c.reply);
+  var marshalled_app_message := MarshallCAppReply(c.reply);
   var marshalled_ep := MarshallEndPoint(c.client);
   val := VTuple([marshalled_ep, VUint64(c.seqno), marshalled_app_message]);
   assert ValInGrammar(val.t[0], CReply_grammar().t[0]);      // OBSERVE 
@@ -871,7 +872,7 @@ method MarshallReplyCache(c:CReplyCache) returns (val:V)
   ensures  |val.a| == |c|
   ensures  ValidVal(val)
   ensures  parse_ReplyCache(val) == c
-  ensures SeqSum(val.a) <= |c| * (8 + (8 + 8) + (24 + max_val_len())); 
+  ensures SeqSum(val.a) <= |c| * (8 + (8 + 8) + (24 + MaxAppReplySize())); 
 {
   if |c| == 0 {
     val := VArray([]);
@@ -908,16 +909,16 @@ method MarshallReplyCache(c:CReplyCache) returns (val:V)
         { reveal SeqSum(); }
       SizeOfV(val.a[0]) + SeqSum(val.a[1..]);
       <=  
-      SizeOfV(val.a[0]) + |remainder| * (8 + (8 + 8) + (24 + max_val_len()));
-      SizeOfV(val.a[0]) + |remainder| * (8 + (8 + 8) + (24 + max_val_len()));
+      SizeOfV(val.a[0]) + |remainder| * (8 + (8 + 8) + (24 + MaxAppReplySize()));
+      SizeOfV(val.a[0]) + |remainder| * (8 + (8 + 8) + (24 + MaxAppReplySize()));
         { lemma_SeqSum2(val.a[0]); }
-      SizeOfV(val.a[0].t[0]) + SizeOfV(val.a[0].t[1]) + |remainder| * (8 + (8 + 8) + (24 + max_val_len()));
+      SizeOfV(val.a[0].t[0]) + SizeOfV(val.a[0].t[1]) + |remainder| * (8 + (8 + 8) + (24 + MaxAppReplySize()));
       <   { lemma_ReplyValValid(c[ep], val.a[0].t[1]); lemma_ReplyBound(c[ep], val.a[0].t[1]); }
-      8 + (8 + 8) + (24 + max_val_len()) + |remainder| * (8 + (8 + 8) + (24 + max_val_len()));
-      1*(8 + (8 + 8) + (24 + max_val_len())) + |remainder| * (8 + (8 + 8) + (24 + max_val_len()));
-        { lemma_mul_is_distributive((8 + (8 + 8) + (24 + max_val_len())), 1, |remainder|); }
-      (1+|remainder|) * (8 + (8 + 8) + (24 + max_val_len()));
-      |c| * (8 + (8 + 8) + (24 + max_val_len()));
+      8 + (8 + 8) + (24 + MaxAppReplySize()) + |remainder| * (8 + (8 + 8) + (24 + MaxAppReplySize()));
+      1*(8 + (8 + 8) + (24 + MaxAppReplySize())) + |remainder| * (8 + (8 + 8) + (24 + MaxAppReplySize()));
+        { lemma_mul_is_distributive((8 + (8 + 8) + (24 + MaxAppReplySize())), 1, |remainder|); }
+      (1+|remainder|) * (8 + (8 + 8) + (24 + MaxAppReplySize()));
+      |c| * (8 + (8 + 8) + (24 + MaxAppReplySize()));
     }
   }
 }
@@ -930,7 +931,7 @@ method{:timeLimitMultiplier 3} MarshallVotes(c:CVotes) returns (val:V)
   ensures  ValidVal(val)
   ensures  parse_Votes(val) == c
   //ensures  val == fun_MarshallVotes(c)
-  ensures SeqSum(val.a) <= |c.v| * (8 + (8 + 8) + (8 + (16 + max_val_len())*RequestBatchSizeLimit()))
+  ensures SeqSum(val.a) <= |c.v| * (8 + (8 + 8) + (8 + (24 + MaxAppRequestSize())*RequestBatchSizeLimit()))
 {
   if |c.v| == 0 {
     val := VArray([]);
@@ -966,18 +967,18 @@ method{:timeLimitMultiplier 3} MarshallVotes(c:CVotes) returns (val:V)
         { reveal SeqSum(); }
       SizeOfV(val.a[0]) + SeqSum(val.a[1..]);
       <=  
-      SizeOfV(val.a[0]) + |remainder| * (8 + (8 + 8) + (8 + ((16 + max_val_len())*RequestBatchSizeLimit())));
-      //SizeOfV(val.a[0]) + |remainder| * (8 + (8 + 8) + (24 + max_val_len()));
+      SizeOfV(val.a[0]) + |remainder| * (8 + (8 + 8) + (8 + ((24 + MaxAppRequestSize())*RequestBatchSizeLimit())));
+      //SizeOfV(val.a[0]) + |remainder| * (8 + (8 + 8) + (24 + MaxAppRequestSize()));
         { lemma_SeqSum2(val.a[0]); }
-      SizeOfV(val.a[0].t[0]) + SizeOfV(val.a[0].t[1]) + |remainder| * (8 + (8 + 8) + (8 + ((16 + max_val_len())*RequestBatchSizeLimit())));
+      SizeOfV(val.a[0].t[0]) + SizeOfV(val.a[0].t[1]) + |remainder| * (8 + (8 + 8) + (8 + ((24 + MaxAppRequestSize())*RequestBatchSizeLimit())));
       <=   { lemma_VoteValValid(c.v[op], val.a[0].t[1]); lemma_VoteBound(c.v[op], val.a[0].t[1]); }
-      8 + (8 + 8) + 8 + ((16 + max_val_len())*|val.a[0].t[1].t[1].a|) + |remainder| * (8 + (8 + 8) + (8 + ((16 + max_val_len())*RequestBatchSizeLimit())));
-      <= { assert |val.a[0].t[1].t[1].a| <= RequestBatchSizeLimit(); lemma_mul_upper_bound(16 + max_val_len(), 16 + max_val_len(), |val.a[0].t[1].t[1].a|, RequestBatchSizeLimit());}
-      8 + (8 + 8) + 8 + ((16 + max_val_len())*RequestBatchSizeLimit()) + |remainder| * (8 + (8 + 8) + (8 + ((16 + max_val_len())*RequestBatchSizeLimit())));
-      1*(8 + (8 + 8) + (8 + ((16 + max_val_len())*RequestBatchSizeLimit()))) + |remainder| * (8 + (8 + 8) + (8 + ((16 + max_val_len())*RequestBatchSizeLimit())));
-        { lemma_mul_is_distributive((8 + (8 + 8) + (8 + ((16 + max_val_len())*RequestBatchSizeLimit()))), 1, |remainder|); }
-      (1+|remainder|) * (8 + (8 + 8) + (8 + ((16 + max_val_len())*RequestBatchSizeLimit())));
-      |c.v| * (8 + (8 + 8) + (8 + ((16 + max_val_len())*RequestBatchSizeLimit())));
+      8 + (8 + 8) + 8 + ((24 + MaxAppRequestSize())*|val.a[0].t[1].t[1].a|) + |remainder| * (8 + (8 + 8) + (8 + ((24 + MaxAppRequestSize())*RequestBatchSizeLimit())));
+      <= { assert |val.a[0].t[1].t[1].a| <= RequestBatchSizeLimit(); lemma_mul_upper_bound(24 + MaxAppRequestSize(), 24 + MaxAppRequestSize(), |val.a[0].t[1].t[1].a|, RequestBatchSizeLimit());}
+      8 + (8 + 8) + 8 + ((24 + MaxAppRequestSize())*RequestBatchSizeLimit()) + |remainder| * (8 + (8 + 8) + (8 + ((24 + MaxAppRequestSize())*RequestBatchSizeLimit())));
+      1*(8 + (8 + 8) + (8 + ((24 + MaxAppRequestSize())*RequestBatchSizeLimit()))) + |remainder| * (8 + (8 + 8) + (8 + ((24 + MaxAppRequestSize())*RequestBatchSizeLimit())));
+        { lemma_mul_is_distributive((8 + (8 + 8) + (8 + ((24 + MaxAppRequestSize())*RequestBatchSizeLimit()))), 1, |remainder|); }
+      (1+|remainder|) * (8 + (8 + 8) + (8 + ((24 + MaxAppRequestSize())*RequestBatchSizeLimit())));
+      |c.v| * (8 + (8 + 8) + (8 + ((24 + MaxAppRequestSize())*RequestBatchSizeLimit())));
     }
   }
 }
@@ -989,7 +990,7 @@ method MarshallMessage_Request(c:CMessage) returns (val:V)
   ensures  ValidVal(val)
   ensures  parse_Message_Request(val) == c
 {
-  var v := MarshallCAppMessage(c.val);
+  var v := MarshallCAppRequest(c.val);
   val := VTuple([VUint64(c.seqno), v]);
 }
 
@@ -1025,11 +1026,10 @@ method MarshallMessage_1b(c:CMessage) returns (val:V)
     SizeOfV(val);
     16 + 8 + SizeOfV(val.t[2]);
     <= 
-    16 + 8 + 8 + (|c.votes.v| * (8 + (8 + 8) + (8 + (16 + max_val_len())*RequestBatchSizeLimit())));
-    32 + (|c.votes.v| * (32 + (16 + 135266329) * 100));
-    32 + (|c.votes.v| * 13526634532);
-    < { lemma_mul_strict_inequality(|c.votes.v|, 8, 13526634532); }
-    32 + (8 * 13526634532);
+    16 + 8 + 8 + (|c.votes.v| * (8 + (8 + 8) + (8 + (24 + MaxAppRequestSize())*RequestBatchSizeLimit())));
+    32 + (|c.votes.v| * (32 + (24 + MaxAppRequestSize()) * 100));
+    < { lemma_mul_strict_inequality(|c.votes.v|, 8, (32 + (24 + MaxAppRequestSize()) * 100)); }
+    32 + (8 * (32 + (24 + MaxAppRequestSize()) * 100));
     <
     MaxPacketSize() - 8;
   }
@@ -1090,7 +1090,7 @@ method MarshallMessage_Reply(c:CMessage) returns (val:V)
   ensures  ValidVal(val)
   ensures  parse_Message_Reply(val) == c
 {
-  var app_val := MarshallCAppMessage(c.reply);
+  var app_val := MarshallCAppReply(c.reply);
   val := VTuple([VUint64(c.seqno_reply), app_val]);
 }
 
@@ -1116,7 +1116,7 @@ method MarshallMessage_AppStateSupply(c:CMessage) returns (val:V)
 {
   var ballot := MarshallBallot(c.bal_state_supply);
   var opn_state_supply := MarshallOperationNumber(c.opn_state_supply);
-  var app_state := MarshallTransferableAppState(c.app_state);
+  var app_state := MarshallCAppState(c.app_state);
   var reply_cache := MarshallReplyCache(c.reply_cache);
   val := VTuple([ballot, opn_state_supply, app_state, reply_cache]);
 
@@ -1125,22 +1125,19 @@ method MarshallMessage_AppStateSupply(c:CMessage) returns (val:V)
   assert ValInGrammar(val.t[0], CBallot_grammar());   // OBSERVE
   lemma_BallotBound(c.bal_state_supply, val.t[0]);
   assert ValInGrammar(val.t[1], COperationNumber_grammar());   // OBSERVE
-  assert ValInGrammar(val.t[2], CTransferableAppState_grammar());    // OBSERVE
-  lemma_TransferableAppStateBound(c.app_state, val.t[2]);
+  assert ValInGrammar(val.t[2], GByteArray);    // OBSERVE
   assert ValInGrammar(val.t[3], CReplyCache_grammar());    // OBSERVE
   calc {
     SizeOfV(val);
     SizeOfV(val.t[0]) + SizeOfV(val.t[1]) + SizeOfV(val.t[2]) + SizeOfV(val.t[3]);
-    <
-    16 + 16 + max_transferable_app_state_size() + SizeOfV(val.t[3]);
     <=
-    16 + 16 + max_transferable_app_state_size() + (8 + |c.reply_cache| * (8 + (8 + 8) + (24 + max_val_len())));  
-    16 + 16 + max_transferable_app_state_size() + (8 + |c.reply_cache| * (8 + (8 + 8) + (24 + 135266329)));  
-    16 + 16 + max_transferable_app_state_size() + (8 + |c.reply_cache| * 135266377); 
-    40 + max_transferable_app_state_size() + |c.reply_cache| * 135266377; 
-    40 + 0x1000_0000_0000_0000 + |c.reply_cache| * 135266377; 
-    < { lemma_mul_strict_inequality(|c.reply_cache|, max_reply_cache_size(), 135266377); }
-    40 + 0x1000_0000_0000_0000 + max_reply_cache_size() * 135266377; 
+    16 + 16 + MaxAppStateSize() + SizeOfV(val.t[3]);
+    <=
+    16 + 16 + MaxAppStateSize() + (8 + |c.reply_cache| * (8 + (8 + 8) + (24 + MaxAppRequestSize())));  
+    16 + 16 + MaxAppStateSize() + (8 + |c.reply_cache| * (MaxAppRequestSize() + 48)); 
+    40 + MaxAppStateSize() + |c.reply_cache| * (MaxAppRequestSize() + 48); 
+    < { lemma_mul_strict_inequality(|c.reply_cache|, max_reply_cache_size(), (MaxAppRequestSize() + 48)); }
+    40 + MaxAppStateSize() + max_reply_cache_size() * (MaxAppRequestSize() + 48); 
     <
     MaxPacketSize() - 8;
   }
@@ -1320,18 +1317,17 @@ lemma lemma_CRequestBound(c:CRequest, val:V)
   requires ValInGrammar(val, CRequest_grammar())
   requires ValidRequest(c)
   requires parse_Request(val) == c
-  ensures  SizeOfV(val) < 16 + max_val_len()
+  ensures  SizeOfV(val) <= 24 + MaxAppRequestSize()
 {
-  ghost var gtuple := GTuple([EndPoint_grammar(), GUint64, CAppMessage_grammar()]);
+  ghost var gtuple := GTuple([EndPoint_grammar(), GUint64, GByteArray]);
   assert ValInGrammar(val, gtuple);
 
   lemma_SeqSum3(val);
-  lemma_AppMessageBound(c.request, val.t[2]);
   assert ValInGrammar(val.t[0], gtuple.t[0]);
   assert ValInGrammar(val.t[1], gtuple.t[1]);
   assert SizeOfV(val.t[0]) == 8;
   assert SizeOfV(val.t[1]) == 8;
-  //assert SizeOfV(val.t[2]) < max_val_len();
+  assert SizeOfV(val.t[2]) <= 8 + MaxAppRequestSize();
 }
 
 lemma lemma_CRequestBatchBound(c:CRequestBatch, val:V)
@@ -1339,25 +1335,25 @@ lemma lemma_CRequestBatchBound(c:CRequestBatch, val:V)
   requires ValidRequestBatch(c)
   requires parse_RequestBatch(val) == c
   decreases |c|
-  ensures  SeqSum(val.a) <= (16 + max_val_len())*|val.a|
+  ensures  SeqSum(val.a) <= (24 + MaxAppRequestSize())*|val.a|
 {
-  //ghost var gtuple := GTuple([EndPoint_grammar(), GUint64, CAppMessage_grammar()]);
+  //ghost var gtuple := GTuple([EndPoint_grammar(), GUint64, GByteArray]);
   ghost var garray := GArray(CRequest_grammar());
   assert ValInGrammar(val, garray);
   reveal SeqSum();
   if |val.a| == 0 {
-    assert SeqSum(val.a) <= (16 + max_val_len())*|val.a|;
+    assert SeqSum(val.a) <= (24 + MaxAppRequestSize())*|val.a|;
   } else {
     var req := parse_Request(val.a[0]);
     var restVal:V := VArray(val.a[1..]);
     var rest := parse_RequestBatch(restVal);
     assert c == [req] + rest;
-    var x := 16 + max_val_len();
+    var x := 24 + MaxAppRequestSize();
     var N := |val.a|;
     lemma_CRequestBatchBound(rest, restVal);
     assert SeqSum(val.a[1..]) <= (x)*(N-1);
     lemma_CRequestBound(req, val.a[0]);
-    assert SizeOfV(val.a[0]) < x;
+    assert SizeOfV(val.a[0]) <= x;
     assert SeqSum(val.a) == SizeOfV(val.a[0]) + SeqSum(val.a[1..]);
     assert |val.a| == |val.a[1..]| + 1;
     lemma_mul_is_distributive(x, N-1, 1);
@@ -1369,17 +1365,16 @@ lemma lemma_ReplyBound(c:CReply, val:V)
   requires ValInGrammar(val, CReply_grammar())
   requires ValidReply(c)
   requires parse_Reply(val) == c
-  ensures  SizeOfV(val) < 24 + max_val_len()
+  ensures  SizeOfV(val) <= 24 + MaxAppRequestSize()
 {
-  ghost var gtuple := GTuple([EndPoint_grammar(), GUint64, CAppMessage_grammar()]);
+  ghost var gtuple := GTuple([EndPoint_grammar(), GUint64, GByteArray]);
   assert ValInGrammar(val, gtuple);
   lemma_SeqSum3(val);
-  lemma_AppMessageBound(c.reply, val.t[2]);
   assert ValInGrammar(val.t[0], gtuple.t[0]);
   assert ValInGrammar(val.t[1], gtuple.t[1]);
   assert SizeOfV(val.t[0]) == 8;
   assert SizeOfV(val.t[1]) == 8;
-  assert SizeOfV(val.t[2]) < max_val_len();
+  assert SizeOfV(val.t[2]) <= 8 + MaxAppRequestSize();
 }
 
 lemma lemma_ReplyValValid(c:CReply, val:V)
@@ -1391,17 +1386,16 @@ lemma lemma_ReplyValValid(c:CReply, val:V)
   lemma_SeqSum3(val);
   assert ValInGrammar(val.t[0], EndPoint_grammar());    // OBSERVE
   assert ValInGrammar(val.t[1], GUint64);    // OBSERVE
-  assert ValInGrammar(val.t[2], CAppMessage_grammar());    // OBSERVE
+  assert ValInGrammar(val.t[2], GByteArray);    // OBSERVE
 
   // Lots of OBSERVE below
-  ghost var gtuple := GTuple([EndPoint_grammar(), GUint64, CAppMessage_grammar()]);
+  ghost var gtuple := GTuple([EndPoint_grammar(), GUint64, GByteArray]);
   assert ValInGrammar(val, gtuple);               
   assert ValInGrammar(val.t[0], gtuple.t[0]);
   assert ValInGrammar(val.t[1], gtuple.t[1]);
   assert ValInGrammar(val.t[2], gtuple.t[2]);
   assert ValidVal(val.t[0]);
   assert ValidVal(val.t[1]);
-  lemma_AppMessageBound(c.reply, val.t[2]);
   assert ValidVal(val.t[2]);
 }
 
@@ -1420,7 +1414,7 @@ lemma {:timeLimitMultiplier 2} lemma_VoteValValid(c:CVote, val:V)
 
   ghost var garray := GArray(CRequest_grammar());
   assert ValInGrammar(val.t[1], garray);
-  ghost var gtuple := GTuple([EndPoint_grammar(), GUint64, CAppMessage_grammar()]);
+  ghost var gtuple := GTuple([EndPoint_grammar(), GUint64, GByteArray]);
   forall i, v | 0 <= i < |val.t[1].a|&& v == val.t[1].a[i]
     ensures ValidVal(v)
   {
@@ -1431,7 +1425,6 @@ lemma {:timeLimitMultiplier 2} lemma_VoteValValid(c:CVote, val:V)
     assert ValidVal(v.t[0]);
     assert ValidVal(v.t[1]);
     assert c.max_val[i] in c.max_val; // OBSERVE antecedent to determine that ValidRequest(c.max_val[i])
-    lemma_AppMessageBound(c.max_val[i].request, v.t[2]);
     assert ValidVal(v.t[2]);
     assert ValidVal(v);
   }
@@ -1456,7 +1449,7 @@ lemma lemma_VoteBound(c:CVote, val:V)
   requires ValidVal(val)
   requires ValidVote(c)
   requires parse_Vote(val) == c
-  ensures  SizeOfV(val) <= (8 + 8) + 8 + ((16 + max_val_len())*|val.t[1].a|)
+  ensures  SizeOfV(val) <= (8 + 8) + 8 + ((24 + MaxAppRequestSize())*|val.t[1].a|)
 {
   lemma_SeqSum2(val);
   assert ValInGrammar(val.t[0], CBallot_grammar());    // OBSERVE
@@ -1477,8 +1470,7 @@ lemma lemma_MarshallableBound(c:CMessage, val:V)
   if c.CMessage_Request? {
     lemma_SeqSum2(val.val);
     assert ValInGrammar(val.val.t[0], GUint64);             // OBSERVE
-    assert ValInGrammar(val.val.t[1], CAppMessage_grammar());    // OBSERVE
-    lemma_AppMessageBound(c.val, val.val.t[1]);
+    assert ValInGrammar(val.val.t[1], GByteArray);    // OBSERVE
   } else if c.CMessage_1a? {
     assert ValInGrammar(val.val, CMessage_1a_grammar());    // OBSERVE
     assert ValInGrammar(val.val, CBallot_grammar());        // OBSERVE
@@ -1497,19 +1489,19 @@ lemma lemma_MarshallableBound(c:CMessage, val:V)
     //assert SizeOfV(val.val.t[2]) == 8 + |val.val.t[2].b| == 8 + |c.val_2a.v|;
     lemma_CRequestBatchBound(c.val_2a, val.val.t[2]);
     assert |val.val.t[2].a| == |c.val_2a|;
+    assert |c.val_2a| <= RequestBatchSizeLimit();
         
     calc {
       SizeOfV(val.val.t[2]);
       8 + SeqSum(val.val.t[2].a);
       <=
-      8 + (16 + max_val_len())*|val.val.t[2].a|;
-      8 + (16 + 135266329)*|val.val.t[2].a|;
-      <
-      MaxPacketSize();
+      8 + (24 + MaxAppRequestSize())*|val.val.t[2].a|;
+      <= { lemma_mul_is_commutative(|val.val.t[2].a|, RequestBatchSizeLimit());
+          lemma_mul_is_commutative(|val.val.t[2].a|, 24 + MaxAppRequestSize());
+          lemma_mul_inequality(|val.val.t[2].a|, RequestBatchSizeLimit(), 24 + MaxAppRequestSize());
+        }
+      8 + (24 + MaxAppRequestSize())*RequestBatchSizeLimit();
     }
-    assert 0 <= SizeOfV(val.val.t[2]) < MaxPacketSize();
-    assert 0 <= SizeOfV(val.val) < MaxPacketSize();
-    assert 0 <= SizeOfV(val) < MaxPacketSize();
   } else if c.CMessage_2b? {
     lemma_SeqSum3(val.val);
     lemma_BallotBound(c.bal_2b, val.val.t[0]);
@@ -1519,6 +1511,17 @@ lemma lemma_MarshallableBound(c:CMessage, val:V)
     assert ValInGrammar(val.val.t[2], CRequestBatch_grammar());    // OBSERVE
     //assert SizeOfV(val.val.t[2]) == 8 + |val.val.t[2].b| == 8 + |c.val_2b.v|;
     lemma_CRequestBatchBound(c.val_2b, val.val.t[2]);
+    calc {
+      SizeOfV(val.val.t[2]);
+      8 + SeqSum(val.val.t[2].a);
+      <=
+      8 + (24 + MaxAppRequestSize())*|val.val.t[2].a|;
+      <= { lemma_mul_is_commutative(|val.val.t[2].a|, RequestBatchSizeLimit());
+          lemma_mul_is_commutative(|val.val.t[2].a|, 24 + MaxAppRequestSize());
+          lemma_mul_inequality(|val.val.t[2].a|, RequestBatchSizeLimit(), 24 + MaxAppRequestSize());
+        }
+      8 + (24 + MaxAppRequestSize())*RequestBatchSizeLimit();
+    }
   } else if c.CMessage_Heartbeat? {
     lemma_SeqSum3(val.val);
     assert ValInGrammar(val.val.t[0], CBallot_grammar());   // OBSERVE
@@ -1527,12 +1530,11 @@ lemma lemma_MarshallableBound(c:CMessage, val:V)
     lemma_BallotBound(c.bal_heartbeat, val.val.t[0]);
   } else if c.CMessage_Reply? {
     lemma_SeqSum2(val.val);
-    assert ValInGrammar(val.val.t[0], GUint64);               // OBSERVE
-    assert ValInGrammar(val.val.t[1], CAppMessage_grammar()); // OBSERVE
-    lemma_AppMessageBound(c.reply, val.val.t[1]);
+    assert ValInGrammar(val.val.t[0], GUint64);     // OBSERVE
+    assert ValInGrammar(val.val.t[1], GByteArray);  // OBSERVE
   } else if c.CMessage_AppStateRequest? {
     lemma_SeqSum2(val.val);
-    assert ValInGrammar(val.val.t[0], CBallot_grammar());   // OBSERVE
+    assert ValInGrammar(val.val.t[0], CBallot_grammar());           // OBSERVE
     assert ValInGrammar(val.val.t[1], COperationNumber_grammar());  // OBSERVE
     lemma_BallotBound(c.bal_state_req, val.val.t[0]);
     assert 0 <= SizeOfV(val) < MaxPacketSize();
