ironfleet/src/Dafny/Distributed/Protocol/RSL/LivenessProof/Assumptions.i.dfy
@@ -16,7 +16,7 @@ import opened Temporal__Temporal_s
 import opened Temporal__Time_s
 import opened Concrete_NodeIdentity_i
 import opened Collections__Maps2_s
-import opened AppStateMachine_i
+import opened AppStateMachine_s
 import opened Environment_s
 import opened Common__UpperBound_s
 
@@ -232,7 +232,7 @@ predicate LivenessAssumptions(
          replica_index in asp.live_quorum ==> HostExecutesPeriodically(b, asp, replica_index))
 
     // The request is valid
-    && AppValidRequest(asp.persistent_request.request)
+    && |asp.persistent_request.request| <= MaxAppRequestSize()
 
     // The persistent client sends its request periodically, with period asp.persistent_period
     && 0 < asp.persistent_period
