ironfleet/src/Dafny/Distributed/Protocol/RSL/Replica.i.dfy
@@ -20,7 +20,7 @@ import opened LiveRSL__Learner_i
 import opened LiveRSL__Executor_i
 import opened LiveRSL__Broadcast_i
 import opened LiveRSL__Message_i
-import opened AppStateMachine_i
+import opened AppStateMachine_s
 import opened Common__UpperBound_s
 import opened Environment_s
 
@@ -53,7 +53,7 @@ predicate LReplicaNextProcessInvalid(s:LReplica, s':LReplica, received_packet:Rs
 predicate LReplicaNextProcessRequest(s:LReplica, s':LReplica, received_packet:RslPacket, sent_packets:seq<RslPacket>)
   requires received_packet.msg.RslMessage_Request?
 {
-  if !AppValidRequest(received_packet.msg.val) then
+  if |received_packet.msg.val| > MaxAppRequestSize() then
     && sent_packets == []
     && s' == s
   else if && received_packet.src in s.executor.reply_cache
